src/program_proof/simplepb/pb_sendcommitthread_proof.v
@@ -2,7 +2,7 @@ From Perennial.program_proof Require Import grove_prelude.
 From Goose.github_com.mit_pdos.gokv.simplepb Require Export pb.
 From Perennial.program_proof.simplepb Require Import pb_protocol.
 From Perennial.goose_lang.lib Require Import waitgroup.
-From Perennial.program_proof.simplepb Require Import pb_definitions pb_increasecommit_proof.
+From Perennial.program_proof.simplepb Require Import pb_definitions pb_increasecommit_proof pb_apply_proof.
 From RecordUpdate Require Import RecordSet.
 Import RecordSetNotations.
 
@@ -19,6 +19,22 @@ Notation pbG := (pbG (pb_record:=pb_record)).
 Notation get_rwops := (get_rwops (pb_record:=pb_record)).
 
 Context `{!pbG Σ}.
+
+Lemma get_commitIndex_facts st γ γsrv :
+  own_Server_ghost_eph_f st γ γsrv -∗
+  ∃ σ,
+  ⌜int.nat st.(server.committedNextIndex) = length σ⌝ ∗
+  is_pb_log_lb γ.(s_pb) σ ∗
+  is_proposal_lb γ.(s_pb) st.(server.epoch) σ ∗
+  □ committed_log_fact γ st.(server.epoch) σ
+.
+Proof.
+  intros.
+  rewrite /own_Server_ghost_eph_f /tc_opaque.
+  iNamed 1.
+  repeat iExists _; iFrame "Hcommit_lb #".
+  iPureIntro. rewrite fmap_length in HcommitLen. word.
+Qed.
 
 Lemma wp_Server__increaseCommitThread (s:loc) γ γsrv :
   {{{
@@ -66,8 +82,130 @@ Proof.
   wp_pures.
   wp_loadField.
   wp_pures.
+  wp_loadField.
 
-  (* This part is just like Apply() *)
-Admitted.
+  iDestruct (get_commitIndex_facts with "HghostEph") as "#Hpre".
+  wp_pures.
+  wp_loadField.
+  wp_apply (release_spec with "[-HΦ]").
+  {
+    iFrame "HmuInv Hlocked".
+    iNext.
+    repeat (iExists _).
+    iSplitR "HghostEph"; last iFrame.
+    repeat (iExists _).
+    iFrame "Hstate ∗#"; iFrame "%".
+  }
+  wp_pures.
+
+  (* XXX: copy paste from Apply proof *)
+  iDestruct "Hprimary" as "[%Hbad|Hprimary]"; first exfalso.
+  { by rewrite Hbad in Heqb. }
+  iNamed "Hprimary".
+  iMod (readonly_load with "Hclerkss_sl") as (?) "Hclerkss_sl2".
+
+  iDestruct (is_slice_small_sz with "Hclerkss_sl2") as %Hclerkss_sz.
+  wp_apply (wp_random).
+  iIntros (randint) "_".
+  wp_apply wp_slice_len.
+  wp_pures.
+  set (clerkIdx:=(word.modu randint clerks_sl.(Slice.sz))).
+
+  assert (int.nat clerkIdx < length clerkss) as Hlookup_clerks.
+  { (* FIXME: better lemmas about mod? *)
+    rewrite Hclerkss_sz.
+    unfold clerkIdx.
+    rewrite Hclerkss_len in Hclerkss_sz.
+    replace (clerks_sl.(Slice.sz)) with (U64 (32)); last first.
+    {
+      unfold numClerks in Hclerkss_sz.
+      word.
+    }
+    enough (int.Z randint `mod` 32 < int.Z 32)%Z.
+    { word. }
+    apply Z.mod_pos_bound.
+    word.
+  }
+
+  assert (∃ clerks_sl_inner, clerkss !! int.nat clerkIdx%Z = Some clerks_sl_inner) as [clerks_sl_inner Hclerkss_lookup].
+  {
+    apply list_lookup_lt.
+    rewrite Hclerkss_len.
+    word.
+  }
+
+  wp_apply (wp_SliceGet with "[$Hclerkss_sl2]").
+  { done. }
+  iIntros "Hclerkss_sl2".
+  wp_pures.
+
+  wp_apply (wp_NewWaitGroup pbN (λ _, True)%I).
+  iIntros (wg γwg) "Hwg".
+  wp_pures.
+
+  iDestruct (big_sepL_lookup_acc with "Hclerkss_rpc") as "[Hclerks_rpc _]".
+  { done. }
+  iNamed "Hclerks_rpc".
+
+  iMod (readonly_load with "Hclerks_sl") as (?) "Hclerks_sl2".
+  iDestruct (is_slice_small_sz with "Hclerks_sl2") as %Hclerks_sz.
+
+  wp_apply (wp_forSlice' _ (λ j, (own_WaitGroup pbN wg γwg j _))%I with "[] [$Hwg $Hclerks_sl2]").
+  2: {
+    iDestruct (big_sepL2_to_sepL_1 with "Hclerks_rpc") as "H2".
+    iFrame "H2".
+  }
+  {
+    iIntros (i ck).
+    simpl.
+    clear Φ.
+    iIntros (Φ) "!# (% & %Hlookup & Hϕ & Hwg) HΦ".
+    iDestruct "Hϕ" as "(% & (% & #Hck & #Hepoch_lb))".
+    wp_pures.
+    wp_apply (wp_WaitGroup__Add with "[$Hwg]").
+    { rewrite Hclerks_sz in H. word. }
+    iIntros "[Hwg Hwg_tok]".
+    wp_pures.
+    iDestruct (own_WaitGroup_to_is_WaitGroup with "[$Hwg]") as "#His_wg".
+    wp_apply (wp_fork with "[Hwg_tok]").
+    {
+      iNext.
+      wp_pures.
+      wp_forBreak_cond.
+      wp_pures.
+
+      iDestruct "Hpre" as (?) "(% & Hlog_lb & Hprop2 & Hcom)".
+      wp_apply (wp_Clerk__IncreaseCommit with "[$Hck]").
+      { iFrame "#%". }
+      iIntros (err) "_".
+
+      wp_pures.
+      wp_if_destruct.
+      2:{
+        wp_pures.
+        iLeft.
+        iFrame "∗".
+        by iPureIntro.
+      }
+      iModIntro.
+      iRight.
+      iSplitR; first done.
+      wp_apply (wp_WaitGroup__Done with "[$Hwg_tok $His_wg]").
+      { done. }
+      done.
+    }
+    iApply "HΦ".
+    iFrame.
+  }
+  iIntros "Hwg".
+  wp_pures.
+  wp_apply (wp_WaitGroup__Wait with "[$]").
+  iIntros "_".
+  wp_pures.
+  wp_apply wp_Sleep.
+  wp_pures.
+  iLeft.
+  by iFrame.
+Qed.
 
 End pb_sendcommitthread_proof.
